project-py/Huffman.py
@@ -1,0 +1,323 @@
+import sys
+from typing import Callable, Any, TypeVar, NamedTuple
+from math import floor
+from itertools import count
+
+import module_ as module_
+import _dafny as _dafny
+import System_ as System_
+
+# Module: Huffman
+
+class default__:
+    def  __init__(self):
+        pass
+
+    @staticmethod
+    def Weight(t):
+        return (t).w
+
+    @staticmethod
+    def PrefixMap(b, m):
+        def iife0_():
+            coll0_ = _dafny.Map()
+            compr_0_: TypeVar('Sym__')
+            for compr_0_ in ((m).keys).Elements:
+                d_0_s_: TypeVar('Sym__') = compr_0_
+                if (d_0_s_) in ((m).keys):
+                    coll0_[d_0_s_] = (_dafny.SeqWithoutIsStrInference([b])) + ((m)[d_0_s_])
+            return _dafny.Map(coll0_)
+        return iife0_()
+        
+
+    @staticmethod
+    def Codes(t):
+        source0_ = t
+        if True:
+            if source0_.is_Leaf:
+                d_0_s_ = source0_.sym
+                return _dafny.Map({d_0_s_: _dafny.SeqWithoutIsStrInference([])})
+        if True:
+            d_1_l_ = source0_.left
+            d_2_r_ = source0_.right
+            return (default__.PrefixMap(False, default__.Codes(d_1_l_))) | (default__.PrefixMap(True, default__.Codes(d_2_r_)))
+
+    @staticmethod
+    def IsPrefix(a, b):
+        def lambda0_(forall_var_0_):
+            d_0_i_: int = forall_var_0_
+            return not (((0) <= (d_0_i_)) and ((d_0_i_) < (len(a)))) or (((a)[d_0_i_]) == ((b)[d_0_i_]))
+
+        return ((len(a)) <= (len(b))) and (_dafny.quantifier(_dafny.IntegerRange(0, len(a)), True, lambda0_))
+
+    @staticmethod
+    def PrefixFreeMap(m):
+        def lambda0_(forall_var_0_):
+            def lambda1_(forall_var_1_):
+                d_1_t_: TypeVar('Sym__') = forall_var_1_
+                return not ((((d_0_s_) in ((m).keys)) and ((d_1_t_) in ((m).keys))) and ((d_0_s_) != (d_1_t_))) or ((not(default__.IsPrefix((m)[d_0_s_], (m)[d_1_t_]))) and (not(default__.IsPrefix((m)[d_1_t_], (m)[d_0_s_]))))
+
+            d_0_s_: TypeVar('Sym__') = forall_var_0_
+            return _dafny.quantifier(((m).keys).Elements, True, lambda1_)
+
+        return _dafny.quantifier(((m).keys).Elements, True, lambda0_)
+
+    @staticmethod
+    def EncodeWithCodes(code, msg):
+        d_0___accumulator_ = _dafny.SeqWithoutIsStrInference([])
+        while True:
+            with _dafny.label():
+                if (len(msg)) == (0):
+                    return (d_0___accumulator_) + (_dafny.SeqWithoutIsStrInference([]))
+                elif True:
+                    d_0___accumulator_ = (d_0___accumulator_) + ((code)[(msg)[0]])
+                    in0_ = code
+                    in1_ = _dafny.SeqWithoutIsStrInference((msg)[1::])
+                    code = in0_
+                    msg = in1_
+                    raise _dafny.TailCall()
+                break
+
+    @staticmethod
+    def Encode(t, msg):
+        return default__.EncodeWithCodes(default__.Codes(t), msg)
+
+    @staticmethod
+    def DecodeOneFrom(node, bits):
+        while True:
+            with _dafny.label():
+                source0_ = node
+                if True:
+                    if source0_.is_Leaf:
+                        d_0_s_ = source0_.sym
+                        return Option_Some((d_0_s_, bits))
+                if True:
+                    d_1_l_ = source0_.left
+                    d_2_r_ = source0_.right
+                    if (len(bits)) == (0):
+                        return Option_None()
+                    elif not((bits)[0]):
+                        in0_ = d_1_l_
+                        in1_ = _dafny.SeqWithoutIsStrInference((bits)[1::])
+                        node = in0_
+                        bits = in1_
+                        raise _dafny.TailCall()
+                    elif True:
+                        in2_ = d_2_r_
+                        in3_ = _dafny.SeqWithoutIsStrInference((bits)[1::])
+                        node = in2_
+                        bits = in3_
+                        raise _dafny.TailCall()
+                break
+
+    @staticmethod
+    def DecodeOptionFuel(t, bits, fuel):
+        if (len(bits)) == (0):
+            return Option_Some(_dafny.SeqWithoutIsStrInference([]))
+        elif (fuel) == (0):
+            return Option_None()
+        elif True:
+            source0_ = default__.DecodeOneFrom(t, bits)
+            if True:
+                if source0_.is_None:
+                    return Option_None()
+            if True:
+                d_0_p_ = source0_.value
+                source1_ = default__.DecodeOptionFuel(t, (d_0_p_)[1], (fuel) - (1))
+                if True:
+                    if source1_.is_None:
+                        return Option_None()
+                if True:
+                    d_1_restMsg_ = source1_.value
+                    return Option_Some((_dafny.SeqWithoutIsStrInference([(d_0_p_)[0]])) + (d_1_restMsg_))
+
+    @staticmethod
+    def DecodeOption(t, bits):
+        return default__.DecodeOptionFuel(t, bits, len(bits))
+
+    @staticmethod
+    def CountOf(msg, x):
+        d_0___accumulator_ = 0
+        while True:
+            with _dafny.label():
+                if (len(msg)) == (0):
+                    return (0) + (d_0___accumulator_)
+                elif True:
+                    d_0___accumulator_ = (d_0___accumulator_) + ((1 if ((msg)[0]) == (x) else 0))
+                    in0_ = _dafny.SeqWithoutIsStrInference((msg)[1::])
+                    in1_ = x
+                    msg = in0_
+                    x = in1_
+                    raise _dafny.TailCall()
+                break
+
+    @staticmethod
+    def DistinctSymbols(msg):
+        syms: _dafny.Seq = _dafny.Seq({})
+        d_0_acc_: _dafny.Seq
+        d_0_acc_ = _dafny.SeqWithoutIsStrInference([])
+        d_1_i_: int
+        d_1_i_ = 0
+        while (d_1_i_) < (len(msg)):
+            if ((msg)[d_1_i_]) in (d_0_acc_):
+                d_1_i_ = (d_1_i_) + (1)
+            elif True:
+                d_2_oldAcc_: _dafny.Seq
+                d_2_oldAcc_ = d_0_acc_
+                d_0_acc_ = (d_2_oldAcc_) + (_dafny.SeqWithoutIsStrInference([(msg)[d_1_i_]]))
+                d_1_i_ = (d_1_i_) + (1)
+        syms = d_0_acc_
+        return syms
+
+    @staticmethod
+    def BuildFreqFromMsg(msg):
+        freq: _dafny.Seq = _dafny.Seq({})
+        d_0_syms_: _dafny.Seq
+        out0_: _dafny.Seq
+        out0_ = default__.DistinctSymbols(msg)
+        d_0_syms_ = out0_
+        freq = _dafny.SeqWithoutIsStrInference([])
+        d_1_i_: int
+        d_1_i_ = 0
+        while (d_1_i_) < (len(d_0_syms_)):
+            d_2_s_: TypeVar('Sym__')
+            d_2_s_ = (d_0_syms_)[d_1_i_]
+            d_3_w_: int
+            d_3_w_ = default__.CountOf(msg, d_2_s_)
+            d_4_oldFreq_: _dafny.Seq
+            d_4_oldFreq_ = freq
+            freq = (d_4_oldFreq_) + (_dafny.SeqWithoutIsStrInference([(d_2_s_, d_3_w_)]))
+            d_1_i_ = (d_1_i_) + (1)
+        return freq
+
+    @staticmethod
+    def BuildHuffmanFromMsg(msg):
+        t: HTree = None
+        d_0_freq_: _dafny.Seq
+        out0_: _dafny.Seq
+        out0_ = default__.BuildFreqFromMsg(msg)
+        d_0_freq_ = out0_
+        out1_: HTree
+        out1_ = default__.BuildHuffman(d_0_freq_)
+        t = out1_
+        return t
+
+    @staticmethod
+    def InsertSorted(q, t):
+        d_0___accumulator_ = _dafny.SeqWithoutIsStrInference([])
+        while True:
+            with _dafny.label():
+                if (len(q)) == (0):
+                    return (d_0___accumulator_) + (_dafny.SeqWithoutIsStrInference([t]))
+                elif (default__.Weight(t)) <= (default__.Weight((q)[0])):
+                    return (d_0___accumulator_) + ((_dafny.SeqWithoutIsStrInference([t])) + (q))
+                elif True:
+                    d_0___accumulator_ = (d_0___accumulator_) + (_dafny.SeqWithoutIsStrInference([(q)[0]]))
+                    in0_ = _dafny.SeqWithoutIsStrInference((q)[1::])
+                    in1_ = t
+                    q = in0_
+                    t = in1_
+                    raise _dafny.TailCall()
+                break
+
+    @staticmethod
+    def CheckPrefixFree(t):
+        ok: bool = False
+        ok = True
+        return ok
+
+    @staticmethod
+    def BuildHuffman(freq):
+        t: HTree = None
+        d_0_q_: _dafny.Seq
+        d_0_q_ = _dafny.SeqWithoutIsStrInference([])
+        d_1_i_: int
+        d_1_i_ = 0
+        while (d_1_i_) < (len(freq)):
+            d_2_s_: TypeVar('Sym__')
+            d_2_s_ = ((freq)[d_1_i_])[0]
+            d_3_w_: int
+            d_3_w_ = ((freq)[d_1_i_])[1]
+            d_4_leaf_: HTree
+            d_4_leaf_ = HTree_Leaf(d_2_s_, d_3_w_)
+            d_5_oldq_: _dafny.Seq
+            d_5_oldq_ = d_0_q_
+            d_0_q_ = default__.InsertSorted(d_5_oldq_, d_4_leaf_)
+            d_1_i_ = (d_1_i_) + (1)
+        while (len(d_0_q_)) > (1):
+            d_6_oldq_: _dafny.Seq
+            d_6_oldq_ = d_0_q_
+            d_7_a_: HTree
+            d_7_a_ = (d_6_oldq_)[0]
+            d_8_b_: HTree
+            d_8_b_ = (d_6_oldq_)[1]
+            d_9_rest_: _dafny.Seq
+            d_9_rest_ = _dafny.SeqWithoutIsStrInference((d_6_oldq_)[2::])
+            d_10_merged_: HTree
+            d_10_merged_ = HTree_Node((default__.Weight(d_7_a_)) + (default__.Weight(d_8_b_)), d_7_a_, d_8_b_)
+            d_11_oldrest_: _dafny.Seq
+            d_11_oldrest_ = d_9_rest_
+            d_0_q_ = default__.InsertSorted(d_11_oldrest_, d_10_merged_)
+        t = (d_0_q_)[0]
+        return t
+
+
+class Option:
+    @classmethod
+    def default(cls, ):
+        return lambda: Option_None()
+    def __ne__(self, __o: object) -> bool:
+        return not self.__eq__(__o)
+    @property
+    def is_None(self) -> bool:
+        return isinstance(self, Option_None)
+    @property
+    def is_Some(self) -> bool:
+        return isinstance(self, Option_Some)
+
+class Option_None(Option, NamedTuple('None_', [])):
+    def __dafnystr__(self) -> str:
+        return f'Huffman.Option.None'
+    def __eq__(self, __o: object) -> bool:
+        return isinstance(__o, Option_None)
+    def __hash__(self) -> int:
+        return super().__hash__()
+
+class Option_Some(Option, NamedTuple('Some', [('value', Any)])):
+    def __dafnystr__(self) -> str:
+        return f'Huffman.Option.Some({_dafny.string_of(self.value)})'
+    def __eq__(self, __o: object) -> bool:
+        return isinstance(__o, Option_Some) and self.value == __o.value
+    def __hash__(self) -> int:
+        return super().__hash__()
+
+
+class HTree:
+    @classmethod
+    def default(cls, default_Sym):
+        return lambda: HTree_Leaf(default_Sym(), int(0))
+    def __ne__(self, __o: object) -> bool:
+        return not self.__eq__(__o)
+    @property
+    def is_Leaf(self) -> bool:
+        return isinstance(self, HTree_Leaf)
+    @property
+    def is_Node(self) -> bool:
+        return isinstance(self, HTree_Node)
+
+class HTree_Leaf(HTree, NamedTuple('Leaf', [('sym', Any), ('w', Any)])):
+    def __dafnystr__(self) -> str:
+        return f'Huffman.HTree.Leaf({_dafny.string_of(self.sym)}, {_dafny.string_of(self.w)})'
+    def __eq__(self, __o: object) -> bool:
+        return isinstance(__o, HTree_Leaf) and self.sym == __o.sym and self.w == __o.w
+    def __hash__(self) -> int:
+        return super().__hash__()
+
+class HTree_Node(HTree, NamedTuple('Node', [('w', Any), ('left', Any), ('right', Any)])):
+    def __dafnystr__(self) -> str:
+        return f'Huffman.HTree.Node({_dafny.string_of(self.w)}, {_dafny.string_of(self.left)}, {_dafny.string_of(self.right)})'
+    def __eq__(self, __o: object) -> bool:
+        return isinstance(__o, HTree_Node) and self.w == __o.w and self.left == __o.left and self.right == __o.right
+    def __hash__(self) -> int:
+        return super().__hash__()
+
