run/__main__.py
@@ -1,9 +1,0 @@
-# Dafny program project.dfy compiled into Python
-import sys
-from typing import Callable, Any, TypeVar, NamedTuple
-from math import floor
-from itertools import count
-
-import run.module_ as module_
-import _dafny as _dafny
-
