project.dfy
@@ -143,9 +143,9 @@ module Huffman {
     }
 
     predicate PrefixFreeMap<Sym>(m: map<Sym, seq<bool>>) {
-    forall s, t | s in m.Keys && t in m.Keys && s != t ::
-      !IsPrefix(m[s], m[t]) && !IsPrefix(m[t], m[s])
-  }
+      forall s, t | s in m.Keys && t in m.Keys && s != t ::
+        !IsPrefix(m[s], m[t]) && !IsPrefix(m[t], m[s])
+    }
 
     lemma PrefixMapPreservesPrefixFree<Sym>(b: bool, m: map<Sym, seq<bool>>)
       requires PrefixFreeMap(m)
@@ -159,7 +159,7 @@ module Huffman {
         var ct := PrefixMap(b, m)[t];
         assert s in m.Keys;
         assert t in m.Keys;
-      
+
         PrefixMapLookup(b, m, s);
         PrefixMapLookup(b, m, t);
 
@@ -169,7 +169,7 @@ module Huffman {
           forall j | 0 <= j < |m[s]|
             ensures m[s][j] == m[t][j]
           {
-            assert cs[j+1] == ct[j+1];   
+            assert cs[j+1] == ct[j+1];
             assert cs[j+1] == m[s][j];
             assert ct[j+1] == m[t][j];
           }
@@ -216,7 +216,7 @@ module Huffman {
         PrefixMapKeys(true, Codes(r));
         assert PrefixMap(false, Codes(l)).Keys == Leaves(l);
         assert PrefixMap(true, Codes(r)).Keys == Leaves(r);
-        assert Leaves(l) !! Leaves(r) by {  
+        assert Leaves(l) !! Leaves(r) by {
           match t
           case Node(_, l, r) => assert Leaves(l) !! Leaves(r);
         }
@@ -226,7 +226,7 @@ module Huffman {
           ensures !IsPrefix(Codes(t)[s], Codes(t)[t']) &&
                   !IsPrefix(Codes(t)[t'], Codes(t)[s])
         {
-          
+
           CodesKeys(t);
           assert s in Leaves(t) && t' in Leaves(t);
           if s in Leaves(l) && t' in Leaves(l) {
@@ -242,7 +242,7 @@ module Huffman {
             assert !IsPrefix(PrefixMap(false, Codes(l))[s], PrefixMap(false, Codes(l))[t']);
             assert !IsPrefix(PrefixMap(false, Codes(l))[t'], PrefixMap(false, Codes(l))[s]);
           } else if s in Leaves(r) && t' in Leaves(r) {
-  
+
             CodesKeys(r);
             PrefixMapKeys(true, Codes(r));
             assert s in Codes(r).Keys && t' in Codes(r).Keys;
@@ -255,9 +255,9 @@ module Huffman {
             assert !IsPrefix(PrefixMap(true, Codes(r))[s], PrefixMap(true, Codes(r))[t']);
             assert !IsPrefix(PrefixMap(true, Codes(r))[t'], PrefixMap(true, Codes(r))[s]);
           } else {
-            
+
             if s in Leaves(l) {
-             
+
               PrefixMapKeys(false, Codes(l));
               PrefixMapKeys(true, Codes(r));
               assert s in PrefixMap(false, Codes(l)).Keys;
@@ -266,14 +266,14 @@ module Huffman {
               MapUnionLookupRight(PrefixMap(false, Codes(l)), PrefixMap(true, Codes(r)), t');
               var cs := Codes(t)[s];
               var ct := Codes(t)[t'];
-              
+
               PrefixMapLookup(false, Codes(l), s);
               PrefixMapLookup(true, Codes(r), t');
               assert cs == [false] + Codes(l)[s];
               assert ct == [true] + Codes(r)[t'];
               assert cs[0] == false;
               assert ct[0] == true;
-              
+
               if IsPrefix(cs, ct) {
                 assert cs[0] == ct[0];
                 assert false;
@@ -283,7 +283,7 @@ module Huffman {
                 assert false;
               }
             } else {
-              
+
               PrefixMapKeys(false, Codes(l));
               PrefixMapKeys(true, Codes(r));
               assert s in PrefixMap(true, Codes(r)).Keys;
@@ -315,7 +315,7 @@ module Huffman {
       requires forall s :: s in msg ==> s in code.Keys
       decreases |msg|
     {
-      if |msg| == 0 then []  
+      if |msg| == 0 then []
       else code[msg[0]] + EncodeWithCodes(code, msg[1..])
     }
 
@@ -326,7 +326,7 @@ module Huffman {
     {
       EncodeWithCodes(Codes(t), msg)
     }
-    
+
     lemma EncodeLenLowerBound<Sym>(t: HTree<Sym>, msg: seq<Sym>)
       requires ValidTree(t) && NonTrivialTree(t)
       requires forall s :: s in msg ==> s in Codes(t).Keys
@@ -453,7 +453,6 @@ module Huffman {
         calc {
           DecodeOptionFuel(t, Encode(t, msg), fuel);
           DecodeOptionFuel(t, Codes(t)[msg[0]] + Encode(t, msg[1..]), fuel);
-          // unfold definition (|bits|>0, fuel>0)
           match DecodeOneFrom(t, Codes(t)[msg[0]] + Encode(t, msg[1..])) {
             case None => None
             case Some(p) => match DecodeOptionFuel(t, p.1, fuel - 1) {
@@ -481,15 +480,15 @@ module Huffman {
       }
     }
 
-  lemma DecodeEncodedRoundTrip<Sym>(t: HTree<Sym>, msg: seq<Sym>)
-    requires ValidTree(t) && NonTrivialTree(t)
-    requires forall s :: s in msg ==> s in Codes(t).Keys
-    ensures DecodeOption(t, Encode(t, msg)) == Some(msg)
-  {
-    var bits := Encode(t, msg);
-    EncodeLenLowerBound(t, msg);
-    RoundTripFuel(t, msg, |bits|);
-  }
+    lemma DecodeEncodedRoundTrip<Sym>(t: HTree<Sym>, msg: seq<Sym>)
+      requires ValidTree(t) && NonTrivialTree(t)
+      requires forall s :: s in msg ==> s in Codes(t).Keys
+      ensures DecodeOption(t, Encode(t, msg)) == Some(msg)
+    {
+      var bits := Encode(t, msg);
+      EncodeLenLowerBound(t, msg);
+      RoundTripFuel(t, msg, |bits|);
+    }
 
     ghost function Alphabet<Sym>(freq: seq<(Sym, nat)>): set<Sym>
       decreases |freq|
@@ -510,393 +509,767 @@ module Huffman {
       forall i :: 0 <= i < |freq| ==> freq[i].1 > 0
     }
 
-    lemma InAlphabetImpliesExists<Sym>(freq: seq<(Sym, nat)>, s: Sym)
-      requires s in Alphabet(freq)
-      ensures exists i :: 0 <= i < |freq| && freq[i].0 == s
-      decreases |freq|
+    ghost function MsgAlphabet<Sym>(msg: seq<Sym>): set<Sym>
+      decreases |msg|
     {
-      if |freq| == 0 {
+      if |msg| == 0 then {}
+      else {msg[0]} + MsgAlphabet(msg[1..])
+    }
+
+    ghost function SeqSet<Sym>(xs: seq<Sym>): set<Sym>
+      decreases |xs|
+    {
+      if |xs| == 0 then {}
+      else {xs[0]} + SeqSet(xs[1..])
+    }
+
+    ghost predicate DistinctSeq<Sym>(xs: seq<Sym>)
+    {
+      forall i, j :: 0 <= i < j < |xs| ==> xs[i] != xs[j]
+    }
+
+    function CountOf<Sym(==)>(msg: seq<Sym>, x: Sym): nat
+      decreases |msg|
+    {
+      if |msg| == 0 then 0
+      else (if msg[0] == x then 1 else 0) + CountOf(msg[1..], x)
+    }
+
+
+    lemma ElementInMsgAlphabet<Sym>(msg: seq<Sym>, s: Sym)
+      requires s in msg
+      ensures s in MsgAlphabet(msg)
+    {
+      if |msg| == 0 {
         assert false;
-      } else if s == freq[0].0 {
-        assert exists i :: 0 <= i < |freq| && freq[i].0 == s by {
-          assert 0 < |freq| && freq[0].0 == s;
-        }
+      } else if msg[0] == s {
       } else {
-        assert s in Alphabet(freq[1..]);
-        InAlphabetImpliesExists(freq[1..], s);
-        var i :| 0 <= i < |freq[1..]| && freq[1..][i].0 == s;
-        assert i+1 < |freq| && freq[i+1].0 == s;
+        assert s in msg[1..];
+        ElementInMsgAlphabet(msg[1..], s);
       }
     }
 
-    lemma DisjointHeadTail<Sym>(freq: seq<(Sym, nat)>)
-      requires DistinctSyms(freq) && |freq| > 0
-      ensures {freq[0].0} !! Alphabet(freq[1..])
-    {
-      if freq[0].0 in Alphabet(freq[1..]) {
-        InAlphabetImpliesExists(freq[1..], freq[0].0);
-        var j :| 0 <= j < |freq[1..]| && freq[1..][j].0 == freq[0].0;
-        assert 0 < j+1 < |freq| && freq[j+1].0 == freq[0].0;
-        assert false by {
-          assert DistinctSyms(freq);
+lemma MsgAlphabetPrefix<Sym>(msg: seq<Sym>, i: nat)
+  requires 0 <= i < |msg|
+  ensures MsgAlphabet(msg[..i+1]) == MsgAlphabet(msg[..i]) + {msg[i]}
+  decreases i
+{
+  if i == 0 {
+    assert msg[..1] == [msg[0]];
+    assert MsgAlphabet([msg[0]]) == {msg[0]};
+    assert MsgAlphabet(msg[..0]) == {};
+  } else {
+    assert msg[..i+1] == [msg[0]] + msg[1..i+1];
+    assert msg[..i] == [msg[0]] + msg[1..i];
+
+    // Apply induction on the tail msg[1..]
+    MsgAlphabetPrefix(msg[1..], i - 1);
+
+    // Help Dafny identify the slices exactly
+    assert (msg[1..])[..i] == msg[1..i+1];
+    assert (msg[1..])[..i-1+1] == msg[1..i+1];
+    assert (msg[1..])[..i-1] == msg[1..i];
+    assert (msg[1..])[i-1] == msg[i];
+
+    assert MsgAlphabet(msg[1..i+1]) == MsgAlphabet(msg[1..i]) + {msg[i]};
+
+    calc {
+      MsgAlphabet(msg[..i+1]);
+      MsgAlphabet([msg[0]] + msg[1..i+1]);
+      { assert MsgAlphabet([msg[0]] + msg[1..i+1]) == ({msg[0]}) + MsgAlphabet(msg[1..i+1]); }
+      ({msg[0]}) + MsgAlphabet(msg[1..i+1]);
+      { assert MsgAlphabet(msg[1..i+1]) == MsgAlphabet(msg[1..i]) + {msg[i]}; }
+      ({msg[0]}) + (MsgAlphabet(msg[1..i]) + {msg[i]});
+      (({msg[0]}) + MsgAlphabet(msg[1..i])) + {msg[i]};
+      { assert ({msg[0]}) + MsgAlphabet(msg[1..i]) == MsgAlphabet(msg[..i]); }
+      MsgAlphabet(msg[..i]) + {msg[i]};
+    }
+  }
+}
+
+lemma SeqSetAppend<Sym>(xs: seq<Sym>, x: Sym)
+  ensures SeqSet(xs + [x]) == SeqSet(xs) + {x}
+  decreases |xs|
+{
+  if |xs| == 0 {
+  } else {
+    assert xs + [x] == [xs[0]] + (xs[1..] + [x]);
+    calc {
+      SeqSet(xs + [x]);
+      SeqSet([xs[0]] + (xs[1..] + [x]));
+      ({xs[0]}) + SeqSet(xs[1..] + [x]);
+      { SeqSetAppend(xs[1..], x); }
+      ({xs[0]}) + (SeqSet(xs[1..]) + {x});
+      ({xs[0]} + SeqSet(xs[1..])) + {x};
+      SeqSet(xs) + {x};
+    }
+  }
+}
+
+lemma IndexInSeqSet<Sym>(xs: seq<Sym>, i: nat)
+  requires 0 <= i < |xs|
+  ensures xs[i] in SeqSet(xs)
+  decreases i
+{
+  if i == 0 {
+  } else {
+    IndexInSeqSet(xs[1..], i - 1);
+  }
+}
+
+lemma DistinctSeqAppendFresh<Sym>(xs: seq<Sym>, x: Sym)
+  requires DistinctSeq(xs)
+  requires x !in SeqSet(xs)
+  ensures DistinctSeq(xs + [x])
+{
+  forall i, j | 0 <= i < j < |xs + [x]|
+    ensures (xs + [x])[i] != (xs + [x])[j]
+  {
+    if j < |xs| {
+      assert xs[i] != xs[j];
+    } else {
+      assert j == |xs|;
+      if i < |xs| {
+        assert (xs + [x])[i] == xs[i];
+        assert (xs + [x])[j] == x;
+        if xs[i] == x {
+          IndexInSeqSet(xs, i);
+          assert xs[i] in SeqSet(xs);
+          assert x in SeqSet(xs);
+          assert false;
         }
       }
     }
+  }
+}
 
-    lemma AlphabetConcat<Sym>(a: seq<(Sym, nat)>, b: seq<(Sym, nat)>)
-      ensures Alphabet(a + b) == Alphabet(a) + Alphabet(b)
-      decreases |a|
+lemma InSeqSetImpliesExists<Sym>(xs: seq<Sym>, x: Sym)
+  requires x in SeqSet(xs)
+  ensures exists j :: 0 <= j < |xs| && xs[j] == x
+  decreases |xs|
+{
+  if |xs| == 0 {
+    assert false;
+  } else {
+    assert SeqSet(xs) == {xs[0]} + SeqSet(xs[1..]);
+    if x == xs[0] {
+      assert exists j :: 0 <= j < |xs| && xs[j] == x by {
+        assert 0 <= 0 < |xs|;
+      }
+    } else {
+      assert x in SeqSet(xs[1..]);
+      InSeqSetImpliesExists(xs[1..], x);
+      var j :| 0 <= j < |xs[1..]| && xs[1..][j] == x;
+      assert xs[j+1] == x;
+      assert exists k :: 0 <= k < |xs| && xs[k] == x by {
+        assert 0 <= j + 1 < |xs|;
+      }
+    }
+  }
+}
+
+lemma DistinctSeqNotInPrefix<Sym>(xs: seq<Sym>, i: nat)
+  requires DistinctSeq(xs)
+  requires 0 <= i < |xs|
+  ensures xs[i] !in SeqSet(xs[..i])
+{
+  if xs[i] in SeqSet(xs[..i]) {
+    InSeqSetImpliesExists(xs[..i], xs[i]);
+    var j :| 0 <= j < |xs[..i]| && xs[..i][j] == xs[i];
+    assert j < i;
+    assert xs[..i][j] == xs[j];
+    assert xs[j] == xs[i];
+    assert false by {
+      assert DistinctSeq(xs);
+    }
+  }
+}
+
+    lemma CountOfPositive<Sym>(msg: seq<Sym>, x: Sym)  // removed (==) because it's ghost
+      requires x in MsgAlphabet(msg)
+      ensures CountOf(msg, x) > 0
+      decreases |msg|
     {
-      if |a| == 0 {
-        assert a + b == b;
-        assert Alphabet(a) == {};
-        assert Alphabet(b) == Alphabet(b);
-        assert Alphabet(a + b) == Alphabet(b);
+      if |msg| == 0 {
+        assert false;
+      } else if msg[0] == x {
+        assert CountOf(msg, x) == 1 + CountOf(msg[1..], x);
       } else {
-        assert a + b == [a[0]] + (a[1..] + b);
-        calc {
-          Alphabet(a + b);
-          Alphabet([a[0]] + (a[1..] + b));
-          { assert Alphabet([a[0]] + (a[1..] + b)) == {a[0].0} + Alphabet(a[1..] + b); }
-          ({a[0].0}) + Alphabet(a[1..] + b);
-          { assert Alphabet(a[1..] + b) == Alphabet(a[1..]) + Alphabet(b); }
-          ({a[0].0}) + (Alphabet(a[1..]) + Alphabet(b));
-          ({a[0].0} + Alphabet(a[1..])) + Alphabet(b);
-          { assert {a[0].0} + Alphabet(a[1..]) == Alphabet(a); }
-          Alphabet(a) + Alphabet(b);
-        }
+        assert x in MsgAlphabet(msg[1..]);
+        CountOfPositive(msg[1..], x);
       }
     }
 
-    lemma AlphabetPrefix<Sym>(freq: seq<(Sym, nat)>, i: nat)
-      requires 0 <= i < |freq|
-      ensures Alphabet(freq[..i+1]) == Alphabet(freq[..i]) + {freq[i].0}
-      decreases i
+    lemma SeqSetSize<Sym>(xs: seq<Sym>)
+      requires DistinctSeq(xs)
+      ensures |SeqSet(xs)| == |xs|
+      decreases |xs|
     {
-      if i == 0 {
-        assert freq[..1] == [freq[0]];
-        assert Alphabet([freq[0]]) == {freq[0].0};
-        assert Alphabet(freq[..0]) == {};
-        assert Alphabet(freq[..1]) == {freq[0].0};
-        assert Alphabet(freq[..0]) + {freq[0].0} == {freq[0].0};
+      if |xs| == 0 {
       } else {
-        assert freq[..i+1] == freq[..i] + [freq[i]];
-        AlphabetConcat(freq[..i], [freq[i]]);
-        assert Alphabet(freq[..i+1]) == Alphabet(freq[..i]) + Alphabet([freq[i]]);
-        assert Alphabet([freq[i]]) == {freq[i].0};
-        assert Alphabet(freq[..i+1]) == Alphabet(freq[..i]) + {freq[i].0};
-      }
-    }
-
-    ghost predicate SortedByWeight<Sym>(q: seq<HTree<Sym>>)
-    {
-      forall i :: 0 <= i < |q| - 1 ==> Weight(q[i]) <= Weight(q[i + 1])
-    }
-
-    ghost function UnionLeaves<Sym>(q: seq<HTree<Sym>>): set<Sym>
-      decreases |q|
-    {
-      if |q| == 0 then {}
-      else Leaves(q[0]) + UnionLeaves(q[1..])
-    }
-
-    ghost predicate DisjointQueue<Sym>(q: seq<HTree<Sym>>)
-      decreases |q|
-    {
-      if |q| <= 1 then true
-      else Leaves(q[0]) !! UnionLeaves(q[1..]) && DisjointQueue(q[1..])
-    }
-
-    ghost predicate QueueInv<Sym>(q: seq<HTree<Sym>>, alphabet: set<Sym>)
-    {
-      |q| >= 1 &&
-      SortedByWeight(q) &&
-      DisjointQueue(q) &&
-      UnionLeaves(q) == alphabet &&
-      forall i :: 0 <= i < |q| ==> ValidTree(q[i])
-    }
-
-    function InsertSorted<Sym(==)>(q: seq<HTree<Sym>>, t: HTree<Sym>): seq<HTree<Sym>>
-      requires SortedByWeight(q)
-      decreases |q|
-    {
-      if |q| == 0 then [t]
-      else if Weight(t) <= Weight(q[0]) then [t] + q
-      else [q[0]] + InsertSorted(q[1..], t)
-    }
-
-    lemma InsertSortedLength<Sym>(q: seq<HTree<Sym>>, t: HTree<Sym>)
-      requires SortedByWeight(q)
-      ensures |InsertSorted(q, t)| == |q| + 1
-    {
-      if |q| == 0 {
-        assert InsertSorted(q, t) == [t];
-      } else if Weight(t) <= Weight(q[0]) {
-        assert InsertSorted(q, t) == [t] + q;
-      } else {
-        assert InsertSorted(q, t) == [q[0]] + InsertSorted(q[1..], t);
-        InsertSortedLength(q[1..], t);
-      }
-    }
-
-    lemma InsertSortedPreservesSorted<Sym>(q: seq<HTree<Sym>>, t: HTree<Sym>)
-      requires SortedByWeight(q)
-      ensures SortedByWeight(InsertSorted(q, t))
-      decreases |q|
-    {
-      if |q| == 0 {
-      } else if Weight(t) <= Weight(q[0]) {
-      } else {
-        InsertSortedPreservesSorted(q[1..], t);
-      }
-    }
-
-    lemma UnionLeavesInsertSorted<Sym>(q: seq<HTree<Sym>>, t: HTree<Sym>)
-      requires SortedByWeight(q)
-      ensures UnionLeaves(InsertSorted(q, t)) == UnionLeaves(q) + Leaves(t)
-      decreases |q|
-    {
-      if |q| == 0 {
-        assert InsertSorted(q, t) == [t];
-      } else if Weight(t) <= Weight(q[0]) {
-        assert InsertSorted(q, t) == [t] + q;
-        calc {
-          UnionLeaves([t] + q);
-          Leaves(t) + UnionLeaves(q);
-        }
-      } else {
-        assert InsertSorted(q, t) == [q[0]] + InsertSorted(q[1..], t);
-        calc {
-          UnionLeaves(InsertSorted(q, t));
-          UnionLeaves([q[0]] + InsertSorted(q[1..], t));
-          Leaves(q[0]) + UnionLeaves(InsertSorted(q[1..], t));
-        }
-        UnionLeavesInsertSorted(q[1..], t);
-        calc {
-          Leaves(q[0]) + (UnionLeaves(q[1..]) + Leaves(t));
-          (Leaves(q[0]) + UnionLeaves(q[1..])) + Leaves(t);
-          UnionLeaves(q) + Leaves(t);
-        }
-      }
-    }
-
-    lemma DisjointQueueInsertSorted<Sym>(q: seq<HTree<Sym>>, t: HTree<Sym>)
-      requires SortedByWeight(q)
-      requires DisjointQueue(q)
-      requires Leaves(t) !! UnionLeaves(q)
-      ensures DisjointQueue(InsertSorted(q, t))
-      decreases |q|
-    {
-      if |q| == 0 {
-      } else if Weight(t) <= Weight(q[0]) {
-      } else {
-        DisjointQueueInsertSorted(q[1..], t);
-        UnionLeavesInsertSorted(q[1..], t);
-        assert UnionLeaves(InsertSorted(q[1..], t)) == UnionLeaves(q[1..]) + Leaves(t);
-        forall x | x in Leaves(q[0]) && x in Leaves(t)
-          ensures false
-        {
-          assert x in UnionLeaves(q) by {
-            assert Leaves(q[0]) <= UnionLeaves(q);
-          }
-          assert false by {
-            assert Leaves(t) !! UnionLeaves(q);
-          }
-        }
-      }
-    }
-
-    lemma InsertSortedPreservesValidity<Sym>(q: seq<HTree<Sym>>, t: HTree<Sym>)
-      requires SortedByWeight(q)
-      requires forall k :: 0 <= k < |q| ==> ValidTree(q[k])
-      requires ValidTree(t)
-      ensures forall k :: 0 <= k < |InsertSorted(q,t)| ==> ValidTree(InsertSorted(q,t)[k])
-      decreases |q|
-    {
-      if |q| == 0 { }
-      else if Weight(t) <= Weight(q[0]) {
-        forall k | 0 <= k < |[t] + q|
-          ensures ValidTree(([t] + q)[k])
-        {
-          if k == 0 {
-            assert ValidTree(t);
-          } else {
-            assert ValidTree(q[k-1]);
-          }
-        }
-      } else {
-        InsertSortedPreservesValidity(q[1..], t);
-        forall k | 0 <= k < |[q[0]] + InsertSorted(q[1..], t)|
-          ensures ValidTree(([q[0]] + InsertSorted(q[1..], t))[k])
-        {
-          if k == 0 {
-            assert ValidTree(q[0]);
-          } else {
-            assert ValidTree(InsertSorted(q[1..], t)[k-1]);
-          }
-        }
-      }
-    }
-
-    lemma AlphabetSize<Sym>(freq: seq<(Sym, nat)>)
-      requires DistinctSyms(freq)
-      ensures |Alphabet(freq)| == |freq|
-    {
-      if |freq| == 0 {
-      } else {
-        DisjointHeadTail(freq);
-        assert Alphabet(freq) == Alphabet([freq[0]]) + Alphabet(freq[1..]) by {
-          assert freq == [freq[0]] + freq[1..];
-          AlphabetConcat([freq[0]], freq[1..]);
-        }
-        assert Alphabet([freq[0]]) == {freq[0].0};
-        AlphabetSize(freq[1..]);
-        assert |Alphabet(freq[1..])| == |freq[1..]|;
-        assert |Alphabet(freq)| == |{freq[0].0} + Alphabet(freq[1..])|;
-        assert {freq[0].0} !! Alphabet(freq[1..]);
-        assert |{freq[0].0} + Alphabet(freq[1..])| == 1 + |Alphabet(freq[1..])|;
-        assert 1 + |Alphabet(freq[1..])| == 1 + |freq[1..]|;
-        assert 1 + |freq[1..]| == |freq|;
-      }
-    }
-
-    method BuildHuffman<Sym(==)>(freq: seq<(Sym, nat)>) returns (t: HTree<Sym>)
-      requires ValidFreq(freq)
-      ensures ValidTree(t)
-      ensures NonTrivialTree(t)
-      ensures Leaves(t) == Alphabet(freq)
-    {
-      var q: seq<HTree<Sym>> := [];
-      var i := 0;
-      while i < |freq|
-        invariant 0 <= i <= |freq|
-        invariant |q| == i
-        invariant SortedByWeight(q)
-        invariant DisjointQueue(q)
-        invariant UnionLeaves(q) == Alphabet(freq[..i])
-        invariant forall k :: 0 <= k < |q| ==> ValidTree(q[k])
-      {
-        var s := freq[i].0;
-        var w := freq[i].1;
-        var leaf := Leaf(s, w);
-        assert ValidTree(leaf);
-
-        assert leaf.sym !in UnionLeaves(q) by {
-          if leaf.sym in UnionLeaves(q) {
-            assert leaf.sym in Alphabet(freq[..i]);
-            InAlphabetImpliesExists(freq[..i], leaf.sym);
-            var j :| 0 <= j < i && freq[..i][j].0 == leaf.sym;
-            assert j < i && freq[j].0 == leaf.sym;
+        assert DistinctSeq(xs[1..]);
+        SeqSetSize(xs[1..]);
+        assert xs[0] !in SeqSet(xs[1..]) by {
+          if xs[0] in SeqSet(xs[1..]) {
+            InSeqSetImpliesExists(xs[1..], xs[0]);
+            var j :| 0 <= j < |xs[1..]| && xs[1..][j] == xs[0];
+            assert xs[j+1] == xs[0];
             assert false by {
-              assert DistinctSyms(freq);
+              assert DistinctSeq(xs);
             }
           }
         }
-
-        var oldq := q;
-        q := InsertSorted(oldq, leaf);
-        InsertSortedPreservesSorted(oldq, leaf);
-        DisjointQueueInsertSorted(oldq, leaf);
-        UnionLeavesInsertSorted(oldq, leaf);
-        InsertSortedPreservesValidity(oldq, leaf);
-        InsertSortedLength(oldq, leaf);
-        assert |q| == |oldq| + 1;
-        assert |oldq| == i;
-        assert |q| == i + 1;
-        AlphabetPrefix(freq, i);
-        assert Alphabet(freq[..i+1]) == Alphabet(freq[..i]) + {freq[i].0};
-        i := i + 1;
+        assert SeqSet(xs) == {xs[0]} + SeqSet(xs[1..]);
+        assert |SeqSet(xs)| == 1 + |SeqSet(xs[1..])|;
+        assert |SeqSet(xs)| == 1 + |xs[1..]|;
+        assert |xs| == 1 + |xs[1..]|;
       }
-
-      assert i == |freq|;
-      assert freq[..i] == freq;
-      assert UnionLeaves(q) == Alphabet(freq);
-      assert |q| >= 2;
-      assert QueueInv(q, Alphabet(freq));
-
-      while |q| > 1
-        invariant QueueInv(q, Alphabet(freq))
-        decreases |q|
-      {
-        var oldq := q;
-        var a := oldq[0];
-        var b := oldq[1];
-        var rest := oldq[2..];
-
-        assert DisjointQueue([b] + rest) by {
-          assert DisjointQueue(oldq) == (Leaves(a) !! UnionLeaves([b] + rest) && DisjointQueue([b] + rest));
-        }
-        assert Leaves(b) !! UnionLeaves(rest) by {
-          assert DisjointQueue([b] + rest) ==> Leaves(b) !! UnionLeaves(rest);
-        }
-
-        var merged := Node(Weight(a) + Weight(b), a, b);
-        assert ValidTree(merged);
-        assert Leaves(merged) == Leaves(a) + Leaves(b);
-        assert Leaves(merged) !! UnionLeaves(rest) by {
-        }
-
-        var oldrest := rest;
-        q := InsertSorted(oldrest, merged);
-        InsertSortedPreservesSorted(oldrest, merged);
-        DisjointQueueInsertSorted(oldrest, merged);
-        UnionLeavesInsertSorted(oldrest, merged);
-        InsertSortedPreservesValidity(oldrest, merged);
-        InsertSortedLength(oldrest, merged);
-        assert |q| == |oldrest| + 1;
-        assert |oldrest| == |oldq| - 2;
-        assert |q| == |oldq| - 1;
-      }
-
-      t := q[0];
-      assert ValidTree(t);
-      assert Leaves(t) == Alphabet(freq) by {
-        assert UnionLeaves(q) == Alphabet(freq);
-        assert |q| == 1 ==> UnionLeaves(q) == Leaves(t);
-      }
-      AlphabetSize(freq);
-      assert |Leaves(t)| == |freq|;
-      assert |freq| >= 2;
-      assert |Leaves(t)| >= 2;
-      assert NonTrivialTree(t);
     }
 
-  lemma HuffmanCorrectness<Sym>(t: HTree<Sym>, msg: seq<Sym>)
-    requires ValidTree(t) && NonTrivialTree(t)
-    requires forall s :: s in msg ==> s in Codes(t).Keys
-    ensures PrefixFreeMap(Codes(t))
-    ensures DecodeOption(t, Encode(t, msg)) == Some(msg)
-  {
-    CodesPrefixFree(t);
-    DecodeEncodedRoundTrip(t, msg);
-  }
-
-
-method {:test} DemoRun()
+lemma InSeqImpliesInSeqSet<Sym>(xs: seq<Sym>, x: Sym)
+  requires x in xs
+  ensures x in SeqSet(xs)
+  decreases |xs|
 {
-  var freq := [('😄', 3), ('C', 6), ('D', 4), ('A', 5), ('E', 2)];
-  var t := BuildHuffman(freq);
+  if |xs| == 0 {
+    assert false;
+  } else if x == xs[0] {
+  } else {
+    assert x in xs[1..];
+    InSeqImpliesInSeqSet(xs[1..], x);
+  }
+}
 
-  CodesKeys(t);
-
-  var msg := ['😄', 'C', 'C','D','A', 'C', 'C','😄','D' ,'A','😄', 'C', 'C','D', 'E', 'A', 'A', 'E', 'D', 'A'];
-
-  assert 'A' in Codes(t).Keys;
-  assert '😄' in Codes(t).Keys;
-  assert 'D' in Codes(t).Keys;
-
-  assert forall s :: s in msg ==> s in Codes(t).Keys by {
-    forall s | s in msg
-      ensures s in Codes(t).Keys
-    {
-      assert s == 'A' || s == '😄' || s=='C'|| s == 'D' || s=='E';
+lemma InSeqSetImpliesInSeq<Sym>(xs: seq<Sym>, x: Sym)
+  requires x in SeqSet(xs)
+  ensures x in xs
+  decreases |xs|
+{
+  if |xs| == 0 {
+    assert false;
+  } else {
+    assert SeqSet(xs) == {xs[0]} + SeqSet(xs[1..]);
+    if x == xs[0] {
+    } else {
+      assert x in SeqSet(xs[1..]);
+      InSeqSetImpliesInSeq(xs[1..], x);
+      assert x in xs[1..];
+      assert x in xs;
     }
   }
+}
 
-  var bits := Encode(t, msg);
-  // print "Encoded bits: ", bits, "\n";
-
-  var decoded := DecodeOption(t, bits);
-  print "Decoded: ", decoded, "\n";
+method DistinctSymbols<Sym(==)>(msg: seq<Sym>) returns (syms: seq<Sym>)
+  ensures DistinctSeq(syms)
+  ensures SeqSet(syms) == MsgAlphabet(msg)
+{
+  var acc: seq<Sym> := [];
+  var i := 0;
+  while i < |msg|
+    invariant 0 <= i <= |msg|
+    invariant DistinctSeq(acc)
+    invariant SeqSet(acc) == MsgAlphabet(msg[..i])
+  {
+    if msg[i] in acc {
+      InSeqImpliesInSeqSet(acc, msg[i]);
+      assert msg[i] in SeqSet(acc);
+      assert msg[i] in MsgAlphabet(msg[..i]);
+      MsgAlphabetPrefix(msg, i);
+      assert MsgAlphabet(msg[..i+1]) == MsgAlphabet(msg[..i]) + {msg[i]};
+      assert MsgAlphabet(msg[..i]) + {msg[i]} == MsgAlphabet(msg[..i]);
+      assert MsgAlphabet(msg[..i+1]) == MsgAlphabet(msg[..i]);
+      i := i + 1;
+    } else {
+  var oldAcc := acc;
+  if msg[i] in SeqSet(oldAcc) {
+    InSeqSetImpliesInSeq(oldAcc, msg[i]);
+    assert msg[i] in oldAcc;
+    assert false;
+  }
+  acc := oldAcc + [msg[i]];
+  DistinctSeqAppendFresh(oldAcc, msg[i]);
+  SeqSetAppend(oldAcc, msg[i]);
+  MsgAlphabetPrefix(msg, i);
+  assert SeqSet(acc) == SeqSet(oldAcc) + {msg[i]};
+  assert SeqSet(acc) == MsgAlphabet(msg[..i]) + {msg[i]};
+  assert MsgAlphabet(msg[..i+1]) == MsgAlphabet(msg[..i]) + {msg[i]};
+  assert SeqSet(acc) == MsgAlphabet(msg[..i+1]);
+  i := i + 1;
 }
   }
+  assert i == |msg|;
+  assert msg[..i] == msg;
+  assert SeqSet(acc) == MsgAlphabet(msg[..i]);
+  assert SeqSet(acc) == MsgAlphabet(msg);
+  syms := acc;
+}
+
+lemma InFreqImpliesInAlphabet<Sym>(freq: seq<(Sym, nat)>, i: nat)
+  requires 0 <= i < |freq|
+  ensures freq[i].0 in Alphabet(freq)
+  decreases |freq|
+{
+  if i == 0 {
+    assert Alphabet(freq) == {freq[0].0} + Alphabet(freq[1..]);
+  } else {
+    InFreqImpliesInAlphabet(freq[1..], i - 1);
+    assert freq[1..][i - 1].0 in Alphabet(freq[1..]);
+    assert freq[1..][i - 1] == freq[i];
+    assert freq[i].0 == freq[1..][i - 1].0;
+    assert Alphabet(freq) == {freq[0].0} + Alphabet(freq[1..]);
+  }
+}
+
+lemma DistinctSymsAppendFresh<Sym>(freq: seq<(Sym, nat)>, s: Sym, w: nat)
+  requires DistinctSyms(freq)
+  requires s !in Alphabet(freq)
+  ensures DistinctSyms(freq + [(s, w)])
+{
+  forall i, j | 0 <= i < j < |freq + [(s, w)]|
+    ensures (freq + [(s, w)])[i].0 != (freq + [(s, w)])[j].0
+  {
+    if j < |freq| {
+      assert freq[i].0 != freq[j].0;
+    } else {
+      assert j == |freq|;
+      if i < |freq| {
+        assert (freq + [(s, w)])[i].0 == freq[i].0;
+        assert (freq + [(s, w)])[j].0 == s;
+        if freq[i].0 == s {
+          InFreqImpliesInAlphabet(freq, i);
+          assert false;
+        }
+      }
+    }
+  }
+}
+
+method BuildFreqFromMsg<Sym(==)>(msg: seq<Sym>) returns (freq: seq<(Sym, nat)>)
+  requires |MsgAlphabet(msg)| >= 2
+  ensures ValidFreq(freq)
+  ensures Alphabet(freq) == MsgAlphabet(msg)
+{
+  var syms := DistinctSymbols(msg);
+  freq := [];
+  var i := 0;
+
+  while i < |syms|
+    invariant 0 <= i <= |syms|
+    invariant |freq| == i
+    invariant DistinctSeq(syms)
+    invariant SeqSet(syms) == MsgAlphabet(msg)
+    invariant DistinctSyms(freq)
+    invariant forall k :: 0 <= k < |freq| ==> freq[k].1 > 0
+    invariant Alphabet(freq) == SeqSet(syms[..i])
+  {
+    var s := syms[i];
+    var w := CountOf(msg, s);
+
+    IndexInSeqSet(syms, i);
+    assert s in SeqSet(syms);
+    assert s in MsgAlphabet(msg);
+    CountOfPositive(msg, s);
+    assert w > 0;
+
+    DistinctSeqNotInPrefix(syms, i);
+    assert s !in SeqSet(syms[..i]);
+    assert s !in Alphabet(freq);
+
+    var oldFreq := freq;
+    freq := oldFreq + [(s, w)];
+
+    DistinctSymsAppendFresh(oldFreq, s, w);
+    AlphabetConcat(oldFreq, [(s, w)]);
+    assert Alphabet([(s, w)]) == {s};
+    assert Alphabet(freq) == Alphabet(oldFreq) + {s};
+    SeqSetAppend(syms[..i], s);
+    assert syms[..i+1] == syms[..i] + [s];
+    assert Alphabet(freq) == SeqSet(syms[..i+1]);
+
+    i := i + 1;
+  }
+
+  assert i == |syms|;
+  assert syms[..i] == syms;
+  assert Alphabet(freq) == SeqSet(syms[..i]);
+  assert Alphabet(freq) == SeqSet(syms);
+  assert Alphabet(freq) == SeqSet(syms);
+  SeqSetSize(syms);
+  assert |SeqSet(syms)| == |syms|;
+  assert |SeqSet(syms)| == |MsgAlphabet(msg)|;
+  assert |syms| >= 2;
+  assert |freq| == |syms|;
+  assert |freq| >= 2;
+}
+
+method BuildHuffmanFromMsg<Sym(==)>(msg: seq<Sym>) returns (t: HTree<Sym>)
+  requires |MsgAlphabet(msg)| >= 2
+  ensures ValidTree(t)
+  ensures NonTrivialTree(t)
+  ensures Leaves(t) == MsgAlphabet(msg)
+{
+  var freq := BuildFreqFromMsg(msg);
+  t := BuildHuffman(freq);
+  assert Alphabet(freq) == MsgAlphabet(msg);
+}
+
+  lemma InAlphabetImpliesExists<Sym>(freq: seq<(Sym, nat)>, s: Sym)
+  requires s in Alphabet(freq)
+  ensures exists i :: 0 <= i < |freq| && freq[i].0 == s
+  decreases |freq|
+  {
+  if |freq| == 0 {
+    assert false;
+  } else if s == freq[0].0 {
+    assert exists i :: 0 <= i < |freq| && freq[i].0 == s by {
+      assert 0 < |freq| && freq[0].0 == s;
+    }
+  } else {
+    assert s in Alphabet(freq[1..]);
+    InAlphabetImpliesExists(freq[1..], s);
+    var i :| 0 <= i < |freq[1..]| && freq[1..][i].0 == s;
+    assert i+1 < |freq| && freq[i+1].0 == s;
+  }
+  }
+
+lemma DisjointHeadTail<Sym>(freq: seq<(Sym, nat)>)
+  requires DistinctSyms(freq) && |freq| > 0
+  ensures {freq[0].0} !! Alphabet(freq[1..])
+{
+  if freq[0].0 in Alphabet(freq[1..]) {
+    InAlphabetImpliesExists(freq[1..], freq[0].0);
+    var j :| 0 <= j < |freq[1..]| && freq[1..][j].0 == freq[0].0;
+    assert 0 < j+1 < |freq| && freq[j+1].0 == freq[0].0;
+    assert false by {
+      assert DistinctSyms(freq);
+    }
+  }
+}
+
+lemma AlphabetConcat<Sym>(a: seq<(Sym, nat)>, b: seq<(Sym, nat)>)
+  ensures Alphabet(a + b) == Alphabet(a) + Alphabet(b)
+  decreases |a|
+{
+  if |a| == 0 {
+    assert a + b == b;
+    assert Alphabet(a) == {};
+    assert Alphabet(b) == Alphabet(b);
+    assert Alphabet(a + b) == Alphabet(b);
+  } else {
+    assert a + b == [a[0]] + (a[1..] + b);
+    calc {
+      Alphabet(a + b);
+      Alphabet([a[0]] + (a[1..] + b));
+      { assert Alphabet([a[0]] + (a[1..] + b)) == {a[0].0} + Alphabet(a[1..] + b); }
+      ({a[0].0}) + Alphabet(a[1..] + b);
+      { assert Alphabet(a[1..] + b) == Alphabet(a[1..]) + Alphabet(b); }
+      ({a[0].0}) + (Alphabet(a[1..]) + Alphabet(b));
+      ({a[0].0} + Alphabet(a[1..])) + Alphabet(b);
+      { assert {a[0].0} + Alphabet(a[1..]) == Alphabet(a); }
+      Alphabet(a) + Alphabet(b);
+    }
+  }
+}
+
+lemma AlphabetPrefix<Sym>(freq: seq<(Sym, nat)>, i: nat)
+  requires 0 <= i < |freq|
+  ensures Alphabet(freq[..i+1]) == Alphabet(freq[..i]) + {freq[i].0}
+  decreases i
+{
+  if i == 0 {
+    assert freq[..1] == [freq[0]];
+    assert Alphabet([freq[0]]) == {freq[0].0};
+    assert Alphabet(freq[..0]) == {};
+    assert Alphabet(freq[..1]) == {freq[0].0};
+    assert Alphabet(freq[..0]) + {freq[0].0} == {freq[0].0};
+  } else {
+    assert freq[..i+1] == freq[..i] + [freq[i]];
+    AlphabetConcat(freq[..i], [freq[i]]);
+    assert Alphabet(freq[..i+1]) == Alphabet(freq[..i]) + Alphabet([freq[i]]);
+    assert Alphabet([freq[i]]) == {freq[i].0};
+    assert Alphabet(freq[..i+1]) == Alphabet(freq[..i]) + {freq[i].0};
+  }
+}
+
+ghost predicate SortedByWeight<Sym>(q: seq<HTree<Sym>>)
+{
+  forall i :: 0 <= i < |q| - 1 ==> Weight(q[i]) <= Weight(q[i + 1])
+}
+
+ghost function UnionLeaves<Sym>(q: seq<HTree<Sym>>): set<Sym>
+  decreases |q|
+{
+  if |q| == 0 then {}
+  else Leaves(q[0]) + UnionLeaves(q[1..])
+}
+
+ghost predicate DisjointQueue<Sym>(q: seq<HTree<Sym>>)
+  decreases |q|
+{
+  if |q| <= 1 then true
+  else Leaves(q[0]) !! UnionLeaves(q[1..]) && DisjointQueue(q[1..])
+}
+
+ghost predicate QueueInv<Sym>(q: seq<HTree<Sym>>, alphabet: set<Sym>)
+{
+  |q| >= 1 &&
+  SortedByWeight(q) &&
+  DisjointQueue(q) &&
+  UnionLeaves(q) == alphabet &&
+  forall i :: 0 <= i < |q| ==> ValidTree(q[i])
+}
+
+function InsertSorted<Sym(==)>(q: seq<HTree<Sym>>, t: HTree<Sym>): seq<HTree<Sym>>
+  requires SortedByWeight(q)
+  decreases |q|
+{
+  if |q| == 0 then [t]
+  else if Weight(t) <= Weight(q[0]) then [t] + q
+  else [q[0]] + InsertSorted(q[1..], t)
+}
+
+lemma InsertSortedLength<Sym>(q: seq<HTree<Sym>>, t: HTree<Sym>)
+  requires SortedByWeight(q)
+  ensures |InsertSorted(q, t)| == |q| + 1
+{
+  if |q| == 0 {
+    assert InsertSorted(q, t) == [t];
+  } else if Weight(t) <= Weight(q[0]) {
+    assert InsertSorted(q, t) == [t] + q;
+  } else {
+    assert InsertSorted(q, t) == [q[0]] + InsertSorted(q[1..], t);
+    InsertSortedLength(q[1..], t);
+  }
+}
+
+lemma InsertSortedPreservesSorted<Sym>(q: seq<HTree<Sym>>, t: HTree<Sym>)
+  requires SortedByWeight(q)
+  ensures SortedByWeight(InsertSorted(q, t))
+  decreases |q|
+{
+  if |q| == 0 {
+  } else if Weight(t) <= Weight(q[0]) {
+  } else {
+    InsertSortedPreservesSorted(q[1..], t);
+  }
+}
+
+lemma UnionLeavesInsertSorted<Sym>(q: seq<HTree<Sym>>, t: HTree<Sym>)
+  requires SortedByWeight(q)
+  ensures UnionLeaves(InsertSorted(q, t)) == UnionLeaves(q) + Leaves(t)
+  decreases |q|
+{
+  if |q| == 0 {
+    assert InsertSorted(q, t) == [t];
+  } else if Weight(t) <= Weight(q[0]) {
+    assert InsertSorted(q, t) == [t] + q;
+    calc {
+      UnionLeaves([t] + q);
+      Leaves(t) + UnionLeaves(q);
+    }
+  } else {
+    assert InsertSorted(q, t) == [q[0]] + InsertSorted(q[1..], t);
+    calc {
+      UnionLeaves(InsertSorted(q, t));
+      UnionLeaves([q[0]] + InsertSorted(q[1..], t));
+      Leaves(q[0]) + UnionLeaves(InsertSorted(q[1..], t));
+    }
+    UnionLeavesInsertSorted(q[1..], t);
+    calc {
+      Leaves(q[0]) + (UnionLeaves(q[1..]) + Leaves(t));
+      (Leaves(q[0]) + UnionLeaves(q[1..])) + Leaves(t);
+      UnionLeaves(q) + Leaves(t);
+    }
+  }
+}
+
+lemma DisjointQueueInsertSorted<Sym>(q: seq<HTree<Sym>>, t: HTree<Sym>)
+  requires SortedByWeight(q)
+  requires DisjointQueue(q)
+  requires Leaves(t) !! UnionLeaves(q)
+  ensures DisjointQueue(InsertSorted(q, t))
+  decreases |q|
+{
+  if |q| == 0 {
+  } else if Weight(t) <= Weight(q[0]) {
+  } else {
+    DisjointQueueInsertSorted(q[1..], t);
+    UnionLeavesInsertSorted(q[1..], t);
+    assert UnionLeaves(InsertSorted(q[1..], t)) == UnionLeaves(q[1..]) + Leaves(t);
+    forall x | x in Leaves(q[0]) && x in Leaves(t)
+      ensures false
+    {
+      assert x in UnionLeaves(q) by {
+        assert Leaves(q[0]) <= UnionLeaves(q);
+      }
+      assert false by {
+        assert Leaves(t) !! UnionLeaves(q);
+      }
+    }
+  }
+}
+
+lemma InsertSortedPreservesValidity<Sym>(q: seq<HTree<Sym>>, t: HTree<Sym>)
+  requires SortedByWeight(q)
+  requires forall k :: 0 <= k < |q| ==> ValidTree(q[k])
+  requires ValidTree(t)
+  ensures forall k :: 0 <= k < |InsertSorted(q,t)| ==> ValidTree(InsertSorted(q,t)[k])
+  decreases |q|
+{
+  if |q| == 0 { }
+  else if Weight(t) <= Weight(q[0]) {
+    forall k | 0 <= k < |[t] + q|
+      ensures ValidTree(([t] + q)[k])
+    {
+      if k == 0 {
+        assert ValidTree(t);
+      } else {
+        assert ValidTree(q[k-1]);
+      }
+    }
+  } else {
+    InsertSortedPreservesValidity(q[1..], t);
+    forall k | 0 <= k < |[q[0]] + InsertSorted(q[1..], t)|
+      ensures ValidTree(([q[0]] + InsertSorted(q[1..], t))[k])
+    {
+      if k == 0 {
+        assert ValidTree(q[0]);
+      } else {
+        assert ValidTree(InsertSorted(q[1..], t)[k-1]);
+      }
+    }
+  }
+}
+
+lemma AlphabetSize<Sym>(freq: seq<(Sym, nat)>)
+  requires DistinctSyms(freq)
+  ensures |Alphabet(freq)| == |freq|
+{
+  if |freq| == 0 {
+  } else {
+    DisjointHeadTail(freq);
+    assert Alphabet(freq) == Alphabet([freq[0]]) + Alphabet(freq[1..]) by {
+      assert freq == [freq[0]] + freq[1..];
+      AlphabetConcat([freq[0]], freq[1..]);
+    }
+    assert Alphabet([freq[0]]) == {freq[0].0};
+    AlphabetSize(freq[1..]);
+    assert |Alphabet(freq[1..])| == |freq[1..]|;
+    assert |Alphabet(freq)| == |{freq[0].0} + Alphabet(freq[1..])|;
+    assert {freq[0].0} !! Alphabet(freq[1..]);
+    assert |{freq[0].0} + Alphabet(freq[1..])| == 1 + |Alphabet(freq[1..])|;
+    assert 1 + |Alphabet(freq[1..])| == 1 + |freq[1..]|;
+    assert 1 + |freq[1..]| == |freq|;
+  }
+}
+
+method CheckPrefixFree<Sym(==)>(t: HTree<Sym>) returns (ok: bool)
+  requires ValidTree(t)
+  ensures ok
+{
+  CodesPrefixFree(t);
+  ok := true;
+}
+
+method BuildHuffman<Sym(==)>(freq: seq<(Sym, nat)>) returns (t: HTree<Sym>)
+requires ValidFreq(freq)
+ensures ValidTree(t)
+ensures NonTrivialTree(t)
+ensures Leaves(t) == Alphabet(freq)
+{
+var q: seq<HTree<Sym>> := [];
+var i := 0;
+while i < |freq|
+  invariant 0 <= i <= |freq|
+  invariant |q| == i
+  invariant SortedByWeight(q)
+  invariant DisjointQueue(q)
+  invariant UnionLeaves(q) == Alphabet(freq[..i])
+  invariant forall k :: 0 <= k < |q| ==> ValidTree(q[k])
+{
+  var s := freq[i].0;
+  var w := freq[i].1;
+  var leaf := Leaf(s, w);
+  assert ValidTree(leaf);
+
+  assert leaf.sym !in UnionLeaves(q) by {
+    if leaf.sym in UnionLeaves(q) {
+      assert leaf.sym in Alphabet(freq[..i]);
+      InAlphabetImpliesExists(freq[..i], leaf.sym);
+      var j :| 0 <= j < i && freq[..i][j].0 == leaf.sym;
+      assert j < i && freq[j].0 == leaf.sym;
+      assert false by {
+        assert DistinctSyms(freq);
+      }
+    }
+  }
+
+  var oldq := q;
+  q := InsertSorted(oldq, leaf);
+  InsertSortedPreservesSorted(oldq, leaf);
+  DisjointQueueInsertSorted(oldq, leaf);
+  UnionLeavesInsertSorted(oldq, leaf);
+  InsertSortedPreservesValidity(oldq, leaf);
+  InsertSortedLength(oldq, leaf);
+  assert |q| == |oldq| + 1;
+  assert |oldq| == i;
+  assert |q| == i + 1;
+  AlphabetPrefix(freq, i);
+  assert Alphabet(freq[..i+1]) == Alphabet(freq[..i]) + {freq[i].0};
+  i := i + 1;
+}
+
+assert i == |freq|;
+assert freq[..i] == freq;
+assert UnionLeaves(q) == Alphabet(freq);
+assert |q| >= 2;
+assert QueueInv(q, Alphabet(freq));
+
+while |q| > 1
+  invariant QueueInv(q, Alphabet(freq))
+  decreases |q|
+{
+  var oldq := q;
+  var a := oldq[0];
+  var b := oldq[1];
+  var rest := oldq[2..];
+
+  assert DisjointQueue([b] + rest) by {
+    assert DisjointQueue(oldq) == (Leaves(a) !! UnionLeaves([b] + rest) && DisjointQueue([b] + rest));
+  }
+  assert Leaves(b) !! UnionLeaves(rest) by {
+    assert DisjointQueue([b] + rest) ==> Leaves(b) !! UnionLeaves(rest);
+  }
+
+  var merged := Node(Weight(a) + Weight(b), a, b);
+  assert ValidTree(merged);
+  assert Leaves(merged) == Leaves(a) + Leaves(b);
+  assert Leaves(merged) !! UnionLeaves(rest) by {
+  }
+
+  var oldrest := rest;
+  q := InsertSorted(oldrest, merged);
+  InsertSortedPreservesSorted(oldrest, merged);
+  DisjointQueueInsertSorted(oldrest, merged);
+  UnionLeavesInsertSorted(oldrest, merged);
+  InsertSortedPreservesValidity(oldrest, merged);
+  InsertSortedLength(oldrest, merged);
+  assert |q| == |oldrest| + 1;
+  assert |oldrest| == |oldq| - 2;
+  assert |q| == |oldq| - 1;
+}
+
+t := q[0];
+assert ValidTree(t);
+assert Leaves(t) == Alphabet(freq) by {
+  assert UnionLeaves(q) == Alphabet(freq);
+  assert |q| == 1 ==> UnionLeaves(q) == Leaves(t);
+}
+AlphabetSize(freq);
+assert |Leaves(t)| == |freq|;
+assert |freq| >= 2;
+assert |Leaves(t)| >= 2;
+assert NonTrivialTree(t);
+}
+
+}
